change ExprCore to depend on Ext/Types
- This will hopefully be temporary, but for the time being
  it makes things much simpler.

src/Ext/ExprCore.v
@@ -1,49 +1,31 @@
 Require Import List Bool.
 Require Import ExtLib.Tactics.Consider.
-Require Import ExtLib.Data.HList.
 Require Import ExtLib.Core.RelDec.
 Require Import ExtLib.Core.Type.
+Require Import ExtLib.Data.HList.
 Require Import ExtLib.Data.Fun.
 Require Import MirrorCore.Generic.
 Require Import MirrorCore.Iso.
-Require Import MirrorCore.TypesI.
 Require Import MirrorCore.EnvI.
 Require Import MirrorCore.ExprI.
+Require Import MirrorCore.Ext.Types.
 
 Set Implicit Arguments.
 Set Strict Implicit.
 
 Section env.
 
-  Variable typ : Type.
-  Variable typD : list Type -> typ -> Type.
-  Context {RType_typ : RType typD}.
-  Context {RTypeOk_typ : RTypeOk RType_typ}.
-  Context {RTypeEq_typ : RTypeEq typD}.
-  Context {RTypeEqOk_typ : RTypeEqOk RType_typ RTypeEq_typ}.
-  Context {typ_arr : TypInstance2 typD Fun}.
-  Context {typ_prop : TypInstance0 typD Prop}.
-  Let tvArr := @typ2 _ _ _ typ_arr.
-  Let arrow_match := @typ2_match _ _ _ typ_arr.
-  Let arrow_in ts a b : (typD ts a -> typD ts b) -> typD ts (tvArr a b) :=
-    @sinto _ _ (@typ2_iso _ _ _ typ_arr ts a b) (fun x => x).
-  Let arrow_out ts a b : typD ts (tvArr a b) -> (typD ts a -> typD ts b) :=
-    @soutof _ _ (@typ2_iso _ _ _ typ_arr ts a b) (fun x => x).
-  Let tvProp := @typ0 _ _ _ typ_prop.
-  Let prop_match := @typ0_match _ _ _ typ_prop.
-  Let prop_in ts : Prop -> typD ts tvProp := 
-    @sinto _ _ (@typ0_iso _ _ _ typ_prop ts) (fun x => x).
-  Let prop_out ts : typD ts tvProp -> Prop := 
-    @soutof _ _ (@typ0_iso _ _ _ typ_prop ts) (fun x => x).
+  Variable types : types.
 
-  Definition typ_cast_val ts (a b : typ) (v : typD ts a) : option (typD ts b) :=
-    match typ_cast (fun x => x) ts a b with
+  Definition typ_cast_val ts (a b : typ) (v : typD types ts a)
+  : option (typD types ts b) :=
+    match typ_cast_typ types (fun x => x) ts a b with
       | None => None
       | Some f => Some (f v)
     end.
 
   Definition func := nat.
-  Record tfunction : Type := 
+  Record tfunction : Type :=
   { tfenv : nat ; tftype : typ }.
   Definition tfunctions := list tfunction.
   Definition var := nat.
@@ -52,7 +34,6 @@ Section env.
   Unset Elimination Schemes.
 
   Inductive expr : Type :=
-  | Const : forall t : typ, typD nil t -> expr
   | Var : var -> expr
   | Func : func -> list typ -> expr
   | App : expr -> list expr -> expr
@@ -75,7 +56,6 @@ Section env.
 
   Section expr_ind.
     Variable P : expr -> Prop.
-    Hypothesis HConst : forall (t : typ) (v : typD nil t), P (@Const t v).
     Hypothesis HVar : forall v : var, P (Var v).
     Hypothesis HFunc : forall f ts, P (Func f ts).
     Hypothesis HUVar : forall v : var, P (UVar v).
@@ -83,12 +63,11 @@ Section env.
     Hypothesis HAbs : forall t e, P e -> P (Abs t e).
     Hypothesis HEqual : forall t e1 e2, P e1 -> P e2 -> P (Equal t e1 e2).
     Hypothesis HNot : forall e, P e -> P (Not e).
-    
+
     Fixpoint expr_ind x : P x.
     Proof.
     refine (
       match x as x return P x with
-        | Const _ _ => HConst _
         | Var _ => HVar _
         | UVar _ => HUVar _
         | Func _ _ => HFunc _ _
@@ -106,12 +85,9 @@ Section env.
 
   Theorem wf_expr_acc : well_founded expr_acc.
   Proof.
-    clear. red. 
-    induction a; simpl; intros; constructor; intros.
-    inversion H.
-    inversion H.
-    inversion H. 
-    inversion H.
+    clear. red.
+    induction a; simpl; intros; constructor; intros;
+    try solve [ inversion H ].
     { inversion H0; clear H0; subst; auto.
       induction es; simpl in *.
       intuition.
@@ -123,32 +99,31 @@ Section env.
   Qed.
 
   Record function := F {
-    fenv : nat ; 
+    fenv : nat ;
     ftype : typ ;
-    fdenote : parametric fenv nil (fun env => typD env ftype)
+    fdenote : parametric fenv nil (fun env => typD types env ftype)
   }.
 
   Definition functions := list function.
   Definition variables := list typ.
 
   Variable funcs : functions.
-  Variable meta_env : env typD.
+  Variable meta_env : env (typD types).
 
   Require Import ExtLib.Data.List.
   Require Import ExtLib.Data.Option.
   Require Import ExtLib.Data.Monads.OptionMonad.
 
   Require Import ExtLib.Structures.Reducible.
-  
+
   Fixpoint typeof (var_env : tenv typ) (e : expr) {struct e} : option typ :=
     match e with
-      | Const t _ => Some t
-      | Var x => 
+      | Var x =>
         match nth_error var_env x with
           | None => None
           | Some tv => Some tv
         end
-      | UVar x => 
+      | UVar x =>
         match nth_error meta_env x with
           | None => None
           | Some tv => Some (projT1 tv)
@@ -156,9 +131,9 @@ Section env.
       | Func f ts =>
         match nth_error funcs f with
           | None => None
-          | Some r => 
+          | Some r =>
 (*            if EqNat.beq_nat (length ts) (fenv r) then  *)
-              Some (instantiate_typ (rev ts) (ftype r))
+              Some (instantiate_typ ts (ftype r))
 (*
             else
               None
@@ -172,7 +147,7 @@ Section env.
                      Monad.bind (typeof var_env e) (type_of_apply tf))
                   (Monad.ret tf) es
         end
-      | Abs t e => 
+      | Abs t e =>
         match typeof (t :: var_env) e with
           | None => None
           | Some t' => Some (tvArr t t')
@@ -180,46 +155,61 @@ Section env.
       | Equal _ _ _ => Some tvProp
       | Not _ => Some tvProp
     end.
-  
-  (** 
+
+  Fixpoint type_apply (n : nat) (ls : list typ) (acc : list Type) (t : typ) {struct n} :
+                 parametric n acc (fun env : list Type => typD types env t) ->
+                 option (typD types acc (instantiate_typ ls t)) :=
+    match n as n , ls as ls
+          return parametric n acc (fun env : list Type => typD types env t) ->
+                 option (typD types acc (instantiate_typ ls t))
+    with
+      | 0 , nil => fun f => Some f
+      | S n , l :: ls => fun f =>
+        match typD_subst0_typ _ _ _ _ in _ = t return option t with
+          | eq_refl =>
+            @type_apply n ls (typD types acc l :: acc) _ (f (typD types acc l))
+        end
+      | _ , _ => fun _ => None
+    end.
+
+  (**
    ** The denotation function with binders must be total because we
    ** can't introduce the binder until we know that we are going to get
    ** the right type out, but, at the same time, we don't know we will
-   ** succeed until after we've taken the denotation of the body, 
+   ** succeed until after we've taken the denotation of the body,
    ** which we can't do until we have the binder.
    **
    **)
-  Fixpoint exprD' (var_env : tenv typ) (e : expr) (t : typ) {struct e} : 
-    option (hlist (typD nil) var_env -> typD nil t).
+  Fixpoint exprD' (var_env : tenv typ) (e : expr) (t : typ) {struct e} :
+    option (hlist (typD types nil) var_env -> typD types nil t).
   refine (
-    match e as e return option (hlist (typD nil) var_env -> typD nil t) with
-      | Const t' c => 
-        match @typ_cast_val _ t' t c with
-          | Some c => Some (fun _ => c)
-          | None => None
-        end
-      | Var x => 
-        match nth_error var_env x as z return z = nth_error var_env x -> option (hlist (typD nil) var_env -> typD nil t) with
+    match e as e return option (hlist (typD types nil) var_env -> typD types nil t) with
+      | Var x =>
+        match nth_error var_env x as z
+          return z = nth_error var_env x ->
+                 option (hlist (typD types nil) var_env -> typD types nil t)
+        with
           | None => fun _ => None
-          | Some t' => fun pf => 
-            match typ_cast (fun x => x) _ t' t with
+          | Some t' => fun pf =>
+            match typ_cast_typ types (fun x => x) _ t' t with
               | Some f =>
                 Some (fun e => match pf in _ = t''
-                                     return match t'' with 
-                                              | Some t => typD nil t
+                                     return match t'' with
+                                              | Some t => typD types nil t
                                               | None => unit
-                                            end -> typD nil t with
+                                            end -> typD types nil t with
                                  | eq_refl => fun x => f x
                                end (hlist_nth e x))
               | None => None
             end
         end eq_refl
-      | UVar x => 
+      | UVar x =>
         match lookupAs meta_env x t with
           | None => None
           | Some v => Some (fun _ => v)
         end
-      | Func f nil =>  
+(*
+      | Func f nil =>
         match nth_error funcs f with
           | None => None
           | Some {| fenv := 0 ; ftype := ft ; fdenote := f |} =>
@@ -227,89 +217,93 @@ Section env.
                        (fun cst => Monad.ret (fun _ => cst f))
           | Some _ => None
         end
+*)
       | Func f ts' =>
-        None (*
         match nth_error funcs f with
           | None => None
           | Some f =>
-            match type_apply _ ts' _ _ (fdenote f) with
+            match type_apply _ ts' _ _ f.(fdenote) with
               | None => None
-              | Some t' => 
-                match @typ_cast_val _ (instantiate_typ (rev ts') (ftype f)) t t' with
+              | Some t' =>
+                match @typ_cast_val _ (instantiate_typ ts' (ftype f)) t t' with
                   | Some v => Some (fun _ => v)
                   | None => None
                 end
             end
-        end *)
+        end
       | Abs t' e =>
-        @arrow_match nil (fun ty Ty => option (hlist (typD nil) var_env -> Ty))
-           (fun lt rt =>
-              match typ_cast (fun x => x) nil lt t' with
-                | None => None
-                | Some cast =>
-                  match @exprD' (lt :: var_env) e rt with
-                    | None => None
-                    | Some a => Some (fun x y => a (Hcons y x))
-                  end
-              end)
-           (fun _ => None)
-           t 
-      | App f xs => 
+        match t as t return option (hlist (typD types nil) var_env -> typD types nil t)
+        with
+          | tvArr lt rt =>
+            match typ_cast_typ types (fun x => x) nil lt t' with
+              | None => None
+              | Some cast =>
+                match @exprD' (lt :: var_env) e rt with
+                  | None => None
+                  | Some a => Some (fun x y => a (Hcons y x))
+                end
+            end
+          | _ => None
+        end
+      | App f xs =>
         match typeof var_env f with
           | None => None
           | Some tf =>
             match exprD' var_env f tf with
               | None => None
               | Some f =>
-                (fix eval_args (t' : typ) (xs : list expr) {struct xs} : 
-                  (hlist (typD nil) var_env -> typD nil t') ->
-                  option (hlist (typD nil) var_env -> typD nil t) :=
+                (fix eval_args (t' : typ) (xs : list expr) {struct xs} :
+                  (hlist (typD types nil) var_env -> typD types nil t') ->
+                  option (hlist (typD types nil) var_env -> typD types nil t) :=
                   match xs with
                     | nil =>
-                      match typ_cast (fun x => x) _ t' t with
+                      match typ_cast_typ types (fun x => x) _ t' t with
                         | None => fun _ => None
                         | Some cast => fun f => Some (fun g => cast (f g))
                       end
-                    | x :: xs => 
-                      @arrow_match nil
-                         (fun ty Ty =>
-                                   (hlist (typD nil) var_env -> Ty) ->
-                            option (hlist (typD nil) var_env -> typD nil t))
-                         (fun tl tr f => 
-                            match exprD' var_env x tl with
-                              | None => None
-                              | Some xv => 
-                                eval_args tr xs (fun e => f e (xv e))
-                            end)
-                         (fun _ _ => None)
-                         t'
+                    | x :: xs =>
+                      match t' as t'
+                        return        (hlist (typD types nil) var_env -> typD types nil t') ->
+                               option (hlist (typD types nil) var_env -> typD types nil t)
+                      with
+                        | tvArr tl tr => fun f =>
+                          match exprD' var_env x tl with
+                            | None => None
+                            | Some xv =>
+                              eval_args tr xs (fun e => f e (xv e))
+                          end
+                        | _ => fun _ => None
+                      end
                   end) tf xs f
             end
         end
       | Equal t' e1 e2 =>
-        @prop_match nil (fun ty Ty => option (hlist (typD nil) var_env -> Ty))
-           (fun _ => 
-              match exprD' var_env e1 t' , exprD' var_env e2 t' with
-                | Some l , Some r => 
-                  Some (fun g => equal (type := typeFor (typD := typD) nil t') (l g) (r g))
-                | _ , _ => None
-              end)
-           (fun _ => None)
-           t
+        match t as t return option (hlist (typD types nil) var_env -> typD types nil t) with
+          | tvProp =>
+            match exprD' var_env e1 t' , exprD' var_env e2 t' with
+              | Some l , Some r =>
+                Some (fun g => (l g) = (r g))
+              (* equal (type := typeFor (typD := typD types) nil t') *)
+              | _ , _ => None
+            end
+          | _ => None
+        end
       | Not e =>
-        @prop_match nil (fun ty Ty => option (hlist (typD nil) var_env -> Ty))
-           (fun _ => 
-              match exprD' var_env e tvProp with
-                | Some P => Some (fun g => not (prop_out (P g)))
-                | _ => None
-              end)
-           (fun _ => None)
-           t
+        match t as t return option (hlist (typD types nil) var_env -> typD types nil t)
+ with
+          | tvProp =>
+            match exprD' var_env e tvProp with
+              | Some P => Some (fun g => not (P g))
+              | _ => None
+            end
+          | _ => None
+        end
     end).
   Defined.
 
-  
-  Definition exprD (var_env : env typD) (e : expr) (t : typ) : option (typD nil t) :=
+
+  Definition exprD (var_env : env (typD types)) (e : expr) (t : typ)
+  : option (typD types nil t) :=
     let (ts,vs) := split_env var_env in
     match exprD' ts e t with
       | None => None
@@ -324,11 +318,10 @@ Section env.
 
   Fixpoint mentionsU (u : nat) (e : expr) {struct e} : bool :=
     match e with
-      | Const _ _ 
-      | Var _ 
+      | Var _
       | Func _ _ => false
       | UVar u' => EqNat.beq_nat u u'
-      | App f es => 
+      | App f es =>
         if mentionsU u f then true else
           (fix anyb ls : bool :=
             match ls with
@@ -340,155 +333,85 @@ Section env.
       | Not e => mentionsU u e
     end.
 
-  Definition const_seqb ts (a b : typ) (x : typD ts a) (y : typD ts b) : option bool :=
+(*
+  Definition const_seqb ts (a b : typ) (x : typD types ts a) (y : typD types ts b)
+  : option bool :=
     match @typ_cast_val ts a b x with
       | None => None
       | Some x' => eqb ts b x' y
     end.
+*)
 
-  Fixpoint expr_seq_dec (e1 e2 : expr) : bool.
+  Fixpoint expr_eq_dec (e1 e2 : expr) : bool.
   refine (
     match e1 , e2 with
-      | Const t1 v1 , Const t2 v2 =>
-        match @const_seqb nil _ _ v1 v2 with
-          | Some x => x
-          | None => false
-        end
       | Var v1 , Var v2 => EqNat.beq_nat v1 v2
       | UVar v1 , UVar v2 => EqNat.beq_nat v1 v2
       | Func f1 ts1 , Func f2 ts2 =>
-        if EqNat.beq_nat f1 f2 then 
-          (fix check ts1 ts2 : bool :=
-            match ts1 , ts2 with
-              | nil , nil => true
-              | t1 :: ts1 , t2 :: ts2 =>
-                if typ_cast (fun x => x) nil t1 t2 then check ts1 ts2 else false
-              | _ , _ => false
-            end) ts1 ts2
+        if EqNat.beq_nat f1 f2 then
+          ts1 ?[ eq ] ts2
         else false
       | App f1 es1 , App f2 es2 =>
-        if expr_seq_dec f1 f2 then
+        if expr_eq_dec f1 f2 then
           (fix check es1 es2 : bool :=
             match es1 , es2 with
               | nil , nil => true
               | e1 :: es1 , e2 :: es2 =>
-                if expr_seq_dec e1 e2 then check es1 es2 else false
+                if expr_eq_dec e1 e2 then check es1 es2 else false
               | _ , _ => false
             end) es1 es2
         else
           false
-      | Abs t1 e1 , Abs t2 e2 => 
-        if typ_cast (fun x => x) nil t1 t2 then expr_seq_dec e1 e2
+      | Abs t1 e1 , Abs t2 e2 =>
+        if t1 ?[ eq ] t2 then expr_eq_dec e1 e2
         else false
       | Equal t1 e1 e2 , Equal t1' e1' e2' =>
-        if typ_cast (fun x => x) nil t1 t1' then 
-          if expr_seq_dec e1 e1' then 
-            if expr_seq_dec e2 e2' then true
+        if t1 ?[ eq ] t1' then
+          if expr_eq_dec e1 e1' then
+            if expr_eq_dec e2 e2' then true
             else false
           else false
         else false
-      | Not e1 , Not e2 => expr_seq_dec e1 e2
+      | Not e1 , Not e2 => expr_eq_dec e1 e2
       | _ , _ => false
     end).
   Defined.
 
-  Theorem const_seqb_ok : forall ts t1 t2 a b,
-    match @const_seqb ts t1 t2 a b with
-      | None => True
-      | Some true => 
-        exists cast : typD ts t2 -> typD ts t1, equal (type := typeFor ts t1) a (cast b)
-      | Some false =>
-        exists cast : typD ts t2 -> typD ts t1, ~equal (type := typeFor ts t1) a (cast b)
-    end.
-  Proof.
-    intros.
-    unfold const_seqb, typ_cast_val. 
-    consider (typ_cast (fun x => x) ts t1 t2); intros; auto.
-    consider (eqb ts t2 (p a) b); intros; auto.
-    specialize (@eqb_ok _ _ _ _ _ ts t2 (p a) b).
-    rewrite H0.
-    destruct (typ_cast_iso (fun x => x) ts t1 t2 H) as [ ? [ ? ? ] ].
-    admit. (*
-    destruct b0; intros.
-    {
-      Check typ_cast_iso.
- destruct (typ_cast_iso (fun x => x) ts t2 t1 H1) as [ ? [ ? ? ] ].
-      specialize (H5 a). specialize (H2 b). 
-      rewrite <- H2 in H3.
-      rewrite H in H4. inversion H4; clear H4; subst. 
-      admit. }
-    { exists x; subst.
-      intro. apply H3; clear H3; subst. admit. } *)
-  Qed.
-
-(*
-  Theorem expr_seq_dec_eq : forall e1 e2, 
-    expr_seq_dec e1 e2 = true -> e1 = e2.
+  Theorem expr_eq_dec_eq : forall e1 e2,
+    expr_eq_dec e1 e2 = true -> e1 = e2.
   Proof.
     induction e1; destruct e2; simpl; intros; try congruence.
-    { generalize (const_seqb_ok t t0 v t1). 
-      destruct (const_seqb t t0 v t1); subst; auto.
-      destruct 1; subst; auto.
-      admit. congruence. }
     { consider (EqNat.beq_nat v v0); subst; auto. }
     { consider (EqNat.beq_nat f f0); intros; subst.
-      f_equal.
-      generalize dependent l; induction ts0; destruct l; simpl in *; try congruence.
-      change typ_eqb with (@rel_dec _ _ _); intros.
-      consider (a ?[ eq ] t); try congruence; intros; subst.
-      f_equal. eapply IHts0; auto. }
+      revert H0.
+      change (ts ?[ eq ] l = true -> Func f0 ts = Func f0 l).
+      consider (ts ?[ eq ] l). intros; subst; reflexivity. }
     { consider (EqNat.beq_nat v u); subst; auto. }
-    { consider (expr_seq_dec e1 e2); intros.
+    { consider (expr_eq_dec e1 e2); intros.
       f_equal; eauto. clear - H1 H.
       generalize dependent l; induction H.
       { destruct l; simpl; auto; try congruence. }
       { destruct l0; simpl; auto; try congruence.
-        consider (expr_seq_dec x e); intros.
+        consider (expr_eq_dec x e); intros.
         f_equal; auto. } }
     { change typ_eqb with (@rel_dec _ _ _) in *. consider (t ?[ eq ] t0).
       intros; subst. f_equal; auto. }
     { change typ_eqb with (@rel_dec _ _ _) in *.
       consider (t ?[ eq ] t0);
-      consider (expr_seq_dec e1_1 e2_1); 
-      consider (expr_seq_dec e1_2 e2_2); intros; subst.
+      consider (expr_eq_dec e1_1 e2_1);
+      consider (expr_eq_dec e1_2 e2_2); intros; subst.
       f_equal; auto. }
     { f_equal; auto. }
   Qed.
-*)  
 
 End env.
 
-Arguments Func {_ _} _ _.
-Arguments Const {_ _} _ _.
-Arguments UVar {_ _} _.
-Arguments Var {_ _} _.
-Arguments Abs {_ _} _ _.
-Arguments App {_ _} _ _.
-
-
 Section expr.
-  Variable typ : Type.
-  Variable typD : list Type -> typ -> Type.
-  Context {RType_typ : RType typD}.
-  Context {RTypeOk_typ : RTypeOk RType_typ}.
-  Context {typ_arr : TypInstance2 typD Fun}.
-  Context {typ_prop : TypInstance0 typD Prop}.
-  Let tvArr := @typ2 _ _ _ typ_arr.
-  Let arrow_match := @typ2_match _ _ _ typ_arr.
-  Let arrow_in ts a b : (typD ts a -> typD ts b) -> typD ts (tvArr a b) :=
-    @sinto _ _ (@typ2_iso _ _ _ typ_arr ts a b) (fun x => x).
-  Let arrow_out ts a b : typD ts (tvArr a b) -> (typD ts a -> typD ts b) :=
-    @soutof _ _ (@typ2_iso _ _ _ typ_arr ts a b) (fun x => x).
-  Let tvProp := @typ0 _ _ _ typ_prop.
-  Let prop_match := @typ0_match _ _ _ typ_prop.
-  Let prop_in ts : Prop -> typD ts tvProp := 
-    @sinto _ _ (@typ0_iso _ _ _ typ_prop ts) (fun x => x).
-  Let prop_out ts : typD ts tvProp -> Prop := 
-    @soutof _ _ (@typ0_iso _ _ _ typ_prop ts) (fun x => x).
+  Variable types : types.
 
-  Instance Expr_expr (fs : functions typD) : Expr typD (expr typD) :=
-  { exprD := @exprD _ _ _ _ _ fs
-  ; acc := @expr_acc _ _
-  ; wf_acc := @wf_expr_acc _ _ 
+  Instance Expr_expr (fs : functions types) : Expr (typD types) expr :=
+  { exprD := exprD fs
+  ; acc := expr_acc
+  ; wf_acc := wf_expr_acc
   }.
 End expr.
